\newpage
\section{Exploration of the covariance given in Eq. (\ref{eq:covariance_g_g})}\label{appendix:B}
In this appendix, we explore the covariance given in Eq. (\ref{eq:covariance_g_g}) to calculate the value more efficiently by computational experiments. Notice that the covariance is written as 
\begin{align}\label{eq:cov_saikei}
	\mathrm{Cov}[g(A_n),\, g(A_{n+k})] 
	= \sum_{i=1}^{\infty} \sum_{j=1}^{\infty} g(i) g(j) \mathrm{Pr} \left[ A_n=i,\,A_{n+k}=j \right] - \{L\times H(\hat{q})\}^2,
\end{align}
where $g$ is given in Eq. (\ref{eq:function_g}), $\mathrm{Pr} \left[ A_n=i,\,A_{n+k}=j \right]$ is given in Eq. (\ref{eq:joint_distribution}), and $H$ is a binary entropy function.
%
Since the term $\{L\times H(\hat{q})\}^2$ is irrelevant to an infinite series, we write the first term of the right hand side (r.h.s.) of Eq. (\ref{eq:cov_saikei}) as
%
\begin{align}\label{eq:Sk}
	\overline{S}_{k} := \sum_{i=1}^{\infty} \sum_{j=1}^{\infty} g(i) g(j) \mathrm{Pr} \left[ A_n=i,\,A_{n+k}=j \right].
\end{align}
%
Firstly, we show the following Lemma concerning an infinite series to calculate the value expressed Eq. (\ref{eq:Sk}). 
%
\begin{lemma}\label{lemma:1}
% abcdefghijklmnopqrstuvwxyz
For any $z \in (0,1)$, the following relation holds
\begin{align}\label{eq:infinite_series}
	\sum_{i=1}^{\infty} g(i) \times (1-z)^i = -\frac{1}{\ln 2} \times \frac{1-z}{z} \times \ln z,
\end{align}
where
\begin{align}
	g(m) = (\log_2 \mathrm{e}) \sum_{k=1}^{m-1} \frac{1}{k}.
\end{align}
\end{lemma}
%-----------------------------------------------------------------------------------------------%
\begin{proof}
Let $t=1-z$, and $\overline{S}$ be the left hand side of Eq. (\ref{eq:infinite_series}), that is,
\begin{align}\begin{split}\label{eq:S}
  \overline{S} &= \sum_{i=1}^{\infty} g(i) \times t^i \\
    % \Leftrightarrow S &= g(1)\times A +  \sum_{i=2}^{\infty} g(i) \times A^{i} \label{eq:S}.
    &= g(1)\times t +  \sum_{i=2}^{\infty} g(i) \times t^{i}.
\end{split}\end{align}
Multiplying the both sides of Eq. (\ref{eq:S}) by $t(\neq 0)$, we obtain the following relation
\begin{align}\begin{split}\label{eq:AS}
  t\times \overline{S} &= \sum_{i=1}^{\infty} g(i) \times t^{i+1} \\
  &= \sum_{i=2}^{\infty} g(i-1) \times t^{i}.
\end{split}\end{align}
Subtracting Eq. (\ref{eq:AS}) from Eq. (\ref{eq:S}), we obtain the following relation
\begin{align}\begin{split}\label{eq:(1-A)S}
  (1-t)\overline{S} &= g(1)\times t^{1} + \sum_{i=2}^{\infty} \left\{ g(i)-g(i-1) \right\} \times t^{i} \\
  &=0 + \sum_{i=2}^{\infty} (\log_2 \mathrm{e}) \times \frac{1}{i-1} \times t^{i} \\
  &=(\log_2 \mathrm{e})\times t \times \sum_{i=1}^{\infty} \frac{t^{i}}{i} \\
  &=(\log_2 \mathrm{e})\times t \times \left\{ - \ln (1-t) \right\}.
\end{split}\end{align}
To obtain the last equality in the above equations, we have used the Taylor series for $|t| < 1$.
Dividing both sides of Eq. (\ref{eq:(1-A)S}) by $1-t (\neq 0)$, we arrive at the following result
\begin{align}
  \overline{S} &= -\frac{1}{\ln 2} \times \frac{t}{1-t} \times \ln (1-t).
\end{align}
The lemma is obtained if we substitute $t$ into $1-z$.
\end{proof}
%-----------------------------------------------------------------------------------------------%
%-----------------------------------------------------------------------------------------------%
%-----------------------------------------------------------------------------------------------%
\par
In the next place, we calculate the value given in Eq. (\ref{eq:Sk}) more in details.
\subsection{Case of $1 \leq j \leq k-1$}
For $1 \leq j \leq k-1$, Eq. (\ref{eq:Sk}) is written as
\begin{align}\begin{split}
  \overline{S}_{k} 
  &:= \sum_{i=1}^{\infty} \sum_{j=1}^{k-1} g(i) g(j) \mathrm{Pr} \left[ A_n=i,\,A_{n+k}=j \right] \\
  &= \sum_{i=1}^{\infty} \sum_{j=1}^{k-1} g(i) g(j) \left( \sum_{r=0}^{L} \binom{L}{r}w_r^2 (1-w_r)^{i-1} \right) \times \left( \sum_{r=0}^{L} \binom{L}{r}w_r^2 (1-w_r)^{j-1} \right) \\ 
  &= \sum_{r=0}^{L} \left\{\binom{L}{r} \frac{w_r^2}{1-w_r} \sum_{i=1}^{\infty} g(i)(1-w_r)^{i} \right\}
  \times \sum_{r=0}^{L} \left\{ \binom{L}{r} \frac{w_r^2}{1-w_r} \sum_{j=1}^{k-1} g(j)(1-w_r)^{j} \right\}.
\end{split}\end{align}
From Lemma \ref{lemma:1}, the infinite series of $i$ in the above equations is written as
\begin{align}
	\sum_{i=1}^{\infty} g(i) (1 - w_r)^{i} = - \frac{1}{\ln 2} \times \frac{1-w_r}{w_r}\times\ln w_r.
\end{align}
%
Therefore, we obtain the following relation
\begin{align}\begin{split}
  \overline{S}_{k}
  =& \sum_{r=0}^{L} \left\{ \dbinom{L}{r} \frac{w_r^2}{1-w_r}  \times \left(- \frac{1}{\ln 2} \times \frac{1-w_r}{w_r}\times\ln w_r \right) \right\} \\
  &\times \sum_{r=0}^{L} \left\{ \dbinom{L}{r} \frac{w_r^2}{1-w_r} \times \sum_{j=1}^{k-1} (1-w_r)^{j} \right\} \\
  =&-\frac{1}{\ln 2}\sum_{r=0}^{L} \left\{ \dbinom{L}{r} w_r \ln w_r \right\} \times \sum_{r=0}^{L} \left\{ \dbinom{L}{r} \frac{w_r^2}{1-w_r} \sum_{j=1}^{k-1} (1-w_r)^{j} \right\}.
\end{split}\end{align}
%
\subsection{Case of $j=k$}
In the case of $j=k$, Eq. (\ref{eq:Sk}) is written as
\begin{align}\begin{split}\label{eq:app_case2}
  \overline{S}_{k} 
  &= \sum_{i=1}^{\infty} g(i) \sum_{r=0}^{L} \binom{L}{r} w_r^3 (1-w_r)^{k+i-2} \sum_{j \in \{k\}} g(j)\\
  &= \sum_{r=0}^{L} \binom{L}{r} w_r^3 (1-w_r)^{k-2} \sum_{i=1}^{\infty} g(i) (1-w_r)^{i} \times g(k) \\
  &= g(k) \times \sum_{r=0}^{L} \binom{L}{r} w_r^3 (1-w_r)^{k-2} \left( -\frac{1}{\ln 2} \times \frac{1-w_{r}}{w_{r}} \times \ln w_{r} \right) \\
  &= -\frac{g(k)}{\ln 2} \times \sum_{r=0}^{L} \binom{L}{r} w_r^2 (1-w_r)^{k-1} \ln w_{r}.
\end{split}\end{align}
The third equation in Eq. (\ref{eq:app_case2}) has been obtained from Lemma \ref{lemma:1}.
%-----------------------------------------------------------------------------------------------%
%-----------------------------------------------------------------------------------------------%
%-----------------------------------------------------------------------------------------------%
\subsection{Case of $k+1 \leq j \leq k+i-1$}
Recall that the joint distribution for $k+1 \leq j \leq k+i-1$ is written as
\begin{align}\begin{split}
	\mathrm{Pr}[A_n=i,\, A_{n+k}=j] 
	=& \sum_{r_1=0}^{L} \sum_{r_2 \neq r_1} \binom{L}{r_1}\binom{L}{r_2}\mathrm{Pr}[e_3(b_1,b_2)] \\
	&+ \sum_{r_1=0}^{L} \sum_{r_2 \in \{r_1\}} \binom{L}{r_1}\left\{\binom{L}{r_1}-1\right\}\mathrm{Pr}[e_3(b_1,b_2)],
\end{split}\end{align}
where $\mathrm{Pr}[e_3(b_1,b_2)]$ is expressed as
\begin{align}\begin{split}
	\mathrm{Pr}[e_3(b_1,b_2)]
  =& w_{r_1}^2  \times w_{r_2}^2 
  \times (1-w_{r_1})^{i-j+k-1} 
  \times (1-w_{r_1}-w_{r_2})^{j-k-1}
  \times (1-w_{r_2})^{k-1} \\
  =&\phi_k(r_1,r_2)\times (1-w_{r_1})^{i} \times \left(1-\frac{w_{r_2}}{1-w_{r_1}} \right)^{j},
\end{split}\end{align}
%
where
\begin{align}\label{eq:phi_k}
	\phi_k(r_1,r_2) = w_{r_1}^2 w_{r_2}^2 
  	(1-w_{r_1})^{k-1} 
  	(1-w_{r_1}-w_{r_2})^{-k-1}
  	(1-w_{r_2})^{k-1}.
\end{align}
%
Then, Eq. (\ref{eq:Sk}) is expressed as
\begin{align}\begin{split}\label{eq:Sk_case3}
	\overline{S}_k 
	=& \sum_{i=1}^{\infty}\sum_{j=k+1}^{k+i-1} g(i)g(j) \sum_{r_1=0}^{L} \sum_{r_2 \neq r_1} \binom{L}{r_1}\binom{L}{r_2}\mathrm{Pr}[e_3(b_1,b_2)]\\ 
	&+ \sum_{i=1}^{\infty}\sum_{j=k+1}^{k+i-1} g(i)g(j) \sum_{r_1=0}^{L} \sum_{r_2 \in \{r_1\}} \binom{L}{r_1} \left\{\binom{L}{r_1}-1 \right\}\mathrm{Pr}[e_3(b_1,b_2)].
\end{split}\end{align}
%
Now, we consider the first term in r.h.s. of Eq. (\ref{eq:Sk_case3}). Let $\overline{A}_1$ be this term of Eq. (\ref{eq:Sk_case3}). We have
\begin{align}\begin{split}\label{eq:A_1}
	\overline{A}_1
	&=\sum_{i=1}^{\infty}\sum_{j=k+1}^{k+i-1} g(i)g(j) \sum_{r_1=0}^{L} \sum_{r_2 \neq r_1} \binom{L}{r_1}\binom{L}{r_2}\mathrm{Pr}[e_3(b_1,b_2)] \\
	&=\sum_{r_1=0}^{L} \sum_{r_2 \neq r_1} \binom{L}{r_1}\binom{L}{r_2}\phi_k(r_1,r_2)
	\sum_{i=1}^{\infty} \sum_{j=1}^{k+i-1} g(i)g(j)(1-w_{r_1})^{i} \times \left(1-\frac{w_{r_2}}{1-w_{r_1}} \right)^{j} \\
	&=\sum_{r_1=0}^{L} \sum_{r_2 \neq r_1} \binom{L}{r_1}\binom{L}{r_2}\phi_k(r_1,r_2)
	\sum_{j=k+1}^{\infty} \sum_{i=k+1}^{k+i-1} g(i)g(j)(1-w_{r_1})^{i} \times \left(1-\frac{w_{r_2}}{1-w_{r_1}} \right)^{j} \\
	&=\sum_{r_1=0}^{L} \sum_{r_2 \neq r_1} \binom{L}{r_1}\binom{L}{r_2}\phi_k(r_1,r_2)
	\sum_{j=k+1}^{\infty} \left\{ g(j) \left(1-\frac{w_{r_2}}{1-w_{r_1}} \right)^{j} \times \sum_{i=j-k+1}^{\infty} g(i)(1-w_{r_1})^{i} \right\}.
\end{split}\end{align}
In the course of the derivation of the above relations, the second equation has been obtained from Eq. (\ref{eq:phi_k}). The third equation has been obtained by exchanging the summation over $i$ and $j$.
%
Then, the infinite series with respect to $i$ in the last equation of Eq. (\ref{eq:A_1}) can be calculated as
\begin{align}\begin{split}
	\sum_{i=j-k+1}^{\infty} g(i)(1-w_{r_1})^{i} 
	&= \sum_{i=1}^{\infty} g(i)(1-w_{r_1})^{i} - \sum_{i=1}^{j-k} g(i)(1-w_{r_1})^{i} \\
	&= -\frac{1}{\ln 2} \times \frac{1-w_{r_1}}{w_{r_1}} \times \ln w_{r_1} - \sum_{i=1}^{j-k} g(i)(1-w_{r_1})^{i}.
\end{split}\end{align}
In the above relations, we have used the result of Lemma \ref{lemma:1}.
Hence, the first term in r.h.s. of Eq. (\ref{eq:Sk_case3}) can be expressed as
\begin{align}
	\overline{A}_1 
	=& \sum_{r_1=0}^{L} \sum_{r_2 \neq r_1} \binom{L}{r_1}\binom{L}{r_2}\phi_k(r_1,r_2)\\
	&\times\sum_{j=k+1}^{\infty} \left[ g(j) \left(1-\frac{w_{r_2}}{1-w_{r_1}} \right)^{j} \times \left\{ -\frac{1}{\ln 2} \times \frac{1-w_{r_1}}{w_{r_1}} \times \ln w_{r_1} - \sum_{i=1}^{j-k} g(i)(1-w_{r_1})^{i} \right\} \right].
\end{align}
We can derive the second term in r.h.s. of Eq. (\ref{eq:Sk_case3}) in the same way as the first term. Let $\overline{A}_2$ be the second term of Eq. (\ref{eq:Sk_case3}). Then, we have
\begin{align}\begin{split}
	\overline{A}_2 =& \sum_{r_1=0}^{L} \sum_{r_2 \in \{r_1\}} \binom{L}{r_1}\left\{\binom{L}{r_1}-1\right\} \phi(r_1,r_2) \\
	&\times\sum_{j=k+1}^{\infty} \left[ g(j) \left(1-\frac{w_{r_2}}{1-w_{r_1}} \right)^{j} \times \left\{ -\frac{1}{\ln 2} \times \frac{1-w_{r_1}}{w_{r_1}} \times \ln w_{r_1} - \sum_{i=1}^{j-k} g(i)(1-w_{r_1})^{i} \right\} \right].
\end{split}\end{align}
%
Therefore, Eq. (\ref{eq:Sk_case3}) can be written as
\begin{align}\begin{split}
	\overline{S}_k =& \overline{A}_1 + \overline{A}_2 \\
	=& \sum_{r_1=0}^{L} \sum_{r_2 \neq r_1} \binom{L}{r_1}\binom{L}{r_2}\phi_k(r_1,r_2)\\
	&\times\sum_{j=k+1}^{\infty} \left[ g(j) \left(1-\frac{w_{r_2}}{1-w_{r_1}} \right)^{j} \times \left\{ -\frac{1}{\ln 2} \times \frac{1-w_{r_1}}{w_{r_1}} \times \ln w_{r_1} - \sum_{i=1}^{j-k} g(i)(1-w_{r_1})^{i} \right\} \right] \\
	&+\sum_{r_1=0}^{L} \sum_{r_2 \in \{r_1\}} \binom{L}{r_1}\left\{\binom{L}{r_1}-1\right\} \phi(r_1,r_2) \\
	&\times\sum_{j=k+1}^{\infty} \left[ g(j) \left(1-\frac{w_{r_2}}{1-w_{r_1}} \right)^{j} \times \left\{ -\frac{1}{\ln 2} 
	\times \frac{1-w_{r_1}}{w_{r_1}} \times \ln w_{r_1} - \sum_{i=1}^{j-k} g(i)(1-w_{r_1})^{i} \right\} \right],
\end{split}\end{align}
where $\phi_k(r_1,r_2)$ is given in Eq. (\ref{eq:phi_k}).
%-----------------------------------------------------------------------------------------------%
%-----------------------------------------------------------------------------------------------%
%-----------------------------------------------------------------------------------------------%
\subsection{Case of $j=k+i$}
Equation (\ref{eq:Sk}) in the case of $j=k+i$ is equal to $0$ from Eq. (\ref{eq:joint_distribution}).
%-----------------------------------------------------------------------------------------------%
%-----------------------------------------------------------------------------------------------%
%-----------------------------------------------------------------------------------------------%
\subsection{Case of $j \geq k+i+1$}
%--------------------------------------------------------------------------------%
Recall that the joint distribution for $j \geq k+i+1$ is written as
\begin{align}\begin{split}
  \mathrm{Pr}[A_n=i,\, A_{n+k}=j] 
  =& \sum_{r_1=0}^{L} \sum_{r_2 \neq r_1} \binom{L}{r_1}\binom{L}{r_2}\mathrm{Pr}[e_5(b_1,b_2)] \\
  &+ \sum_{r_1=0}^{L} \sum_{r_2 \in \{r_1\}} \binom{L}{r_1}\left\{\binom{L}{r_1}-1\right\}\mathrm{Pr}[e_5(b_1,b_2)],
\end{split}\end{align}
where $\mathrm{Pr}[e_5(b_1,b_2)]$ is expressed as
\begin{align}\begin{split}
  \mathrm{Pr}[e_5(b_1,b_2)]
  =& w_{r_1}^2  \times w_{r_2}^2 
  \times (1-w_{r_1})^{-i+j-k-1} 
  \times (1-w_{r_1}-w_{r_2})^{i-1}
  \times (1-w_{r_1})^{k-1} \\
  =&\psi_k(r_1,r_2)\times \left(1-\frac{w_{r_2}}{1-w_{r_1}} \right)^{i} \times (1-w_{r_1})^j,
\end{split}\end{align}
%
where
\begin{align}\begin{split}\label{eq:psi_k}
  \psi_k(r_1,r_2) 
  &= w_{r_1}^2 w_{r_2}^2 
    (1-w_{r_1})^{-k-1} 
    (1-w_{r_1}-w_{r_2})^{-1}
    (1-w_{r_1})^{k-1} \\
  &= w_{r_1}^2 w_{r_2}^2 (1-w_{r_1})^{-2} (1-w_{r_1}-w_{r_2})^{-1}.
\end{split}\end{align}
%
Then, Eq. (\ref{eq:Sk}) is expressed as
\begin{align}\begin{split}\label{eq:Sk_case5}
  \overline{S}_k 
  =& \sum_{i=1}^{\infty}\sum_{j=k+i+1}^{\infty} g(i)g(j) \sum_{r_1=0}^{L} \sum_{r_2 \neq r_1} \binom{L}{r_1}\binom{L}{r_2}\mathrm{Pr}[e_5(b_1,b_2)]\\ 
  &+ \sum_{i=1}^{\infty}\sum_{j=k+i+1}^{\infty} g(i)g(j) \sum_{r_1=0}^{L} \sum_{r_2 \in \{r_1\}} \binom{L}{r_1} \left\{\binom{L}{r_1}-1 \right\}\mathrm{Pr}[e_5(b_1,b_2)].
\end{split}\end{align}
%
Firstly, we consider the first term in the r.h.s. of Eq. (\ref{eq:Sk_case3}). Let $\overline{B}_1$ be the first term of Eq. (\ref{eq:Sk_case3}). Then, $\overline{B}_1$ is written as
\begin{align}\begin{split}\label{eq:B_1}
  \overline{B}_1
  &=\sum_{i=1}^{\infty}\sum_{j=k+i+1}^{\infty} g(i)g(j) \sum_{r_1=0}^{L} \sum_{r_2 \neq r_1} \binom{L}{r_1}\binom{L}{r_2}\mathrm{Pr}[e_5(b_1,b_2)] \\
  &=\sum_{r_1=0}^{L} \sum_{r_2 \neq r_1} \binom{L}{r_1}\binom{L}{r_2}\psi_k(r_1,r_2)
  \sum_{i=1}^{\infty} \sum_{j=k+i+1}^{\infty} g(i)g(j) \left(1-\frac{w_{r_2}}{1-w_{r_1}} \right)^{i} \times (1-w_{r_1})^j \\
  &=\sum_{r_1=0}^{L} \sum_{r_2 \neq r_1} \binom{L}{r_1}\binom{L}{r_2}\psi_k(r_1,r_2)
  \sum_{i=1}^{\infty} g(i)\left(1-\frac{w_{r_2}}{1-w_{r_1}} \right)^{i} \times \sum_{j=k+i+1}^{\infty} g(j) (1-w_{r_1})^j.
\end{split}\end{align}
In the course of the derivation of the above relations, the second equation has been obtained from Eq. (\ref{eq:phi_k}). The third equation has been obtained by exchange of infinite series.
%
Then, the infinite sum with respect to $j$ in the last equation of Eq. (\ref{eq:B_1}) can be calculated as
\begin{align}\begin{split}
  \sum_{j=k+i+1}^{\infty} g(j) (1-w_{r_1})^j 
  &= \sum_{j=1}^{\infty} g(j)(1-w_{r_1})^{j} - \sum_{j=1}^{k+i} g(j)(1-w_{r_1})^{j} \\
  &= -\frac{1}{\ln 2} \times \frac{1-w_{r_1}}{w_{r_1}} \times \ln w_{r_1} - \sum_{j=1}^{k+i} g(j)(1-w_{r_1})^{j}.
\end{split}\end{align}
In the above relations, we use the result of Lemma \ref{lemma:1}.
Hence, the first term of Eq. (\ref{eq:Sk_case5}) can be expressed as
\begin{align}
  \overline{B}_1 
  =& \sum_{r_1=0}^{L} \sum_{r_2 \neq r_1} \binom{L}{r_1}\binom{L}{r_2}\psi_k(r_1,r_2)\\
  &\times\sum_{i=1}^{\infty} \left[ g(i) \left(1-\frac{w_{r_2}}{1-w_{r_1}} \right)^{i} \times \left\{ -\frac{1}{\ln 2} \times \frac{1-w_{r_1}}{w_{r_1}} \times \ln w_{r_1} - \sum_{j=1}^{k+i} g(j)(1-w_{r_1})^{j} \right\} \right].
\end{align}
We can derive the second term of Eq. (\ref{eq:Sk_case5}) in the same way as the first term. Let $\overline{B}_2$ be the second term of Eq. (\ref{eq:Sk_case5}). Then, we have
\begin{align}\begin{split}
  \overline{B}_2 =& \sum_{r_1=0}^{L} \sum_{r_2 \in \{r_1\}} \binom{L}{r_1}\left\{\binom{L}{r_1}-1\right\} \psi(r_1,r_2) \\
  &\times\sum_{i=1}^{\infty} \left[ g(i) \left(1-\frac{w_{r_2}}{1-w_{r_1}} \right)^{i} \times \left\{ -\frac{1}{\ln 2} \times \frac{1-w_{r_1}}{w_{r_1}} \times \ln w_{r_1} - \sum_{j=1}^{k+i} g(j)(1-w_{r_1})^{j} \right\} \right].
\end{split}\end{align}
%
Therefore, Eq. (\ref{eq:Sk_case5}) can be expressed as
\begin{align}\begin{split}
  \overline{S}_k =& \overline{B}_1 + \overline{B}_2 \\
  =& \sum_{r_1=0}^{L} \sum_{r_2 \neq r_1} \binom{L}{r_1}\binom{L}{r_2}\psi_k(r_1,r_2)\\
  &\times\sum_{i=1}^{\infty} \left[ g(i) \left(1-\frac{w_{r_2}}{1-w_{r_1}} \right)^{i} \times \left\{ -\frac{1}{\ln 2} \times \frac{1-w_{r_1}}{w_{r_1}} \times \ln w_{r_1} - \sum_{j=1}^{k+i} g(j)(1-w_{r_1})^{j} \right\} \right] \\
  &+\sum_{r_1=0}^{L} \sum_{r_2 \in \{r_1\}} \binom{L}{r_1}\left\{\binom{L}{r_1}-1\right\} \psi(r_1,r_2) \\
  &\times\sum_{i=1}^{\infty} \left[ g(i) \left(1-\frac{w_{r_2}}{1-w_{r_1}} \right)^{i} \times \left\{ -\frac{1}{\ln 2} \times \frac{1-w_{r_1}}{w_{r_1}} \times \ln w_{r_1} - \sum_{j=1}^{k+i} g(j)(1-w_{r_1})^{j} \right\} \right],
\end{split}\end{align}
where $\psi_k(r_1,r_2)$ is given in Eq. (\ref{eq:psi_k}).


















